src/Examples/Logging2/Liftable.v
@@ -1,0 +1,204 @@
+From iris.algebra Require Import auth gmap list.
+Require Export CSL.Refinement CSL.NamedDestruct.
+Require Import ExMach.WeakestPre ExMach.RefinementAdequacy.
+Require Import Equality.
+Set Default Proof Using "All".
+Unset Implicit Arguments.
+
+
+Notation "l ↦[ t ] v " := (mapsto (hG := t) l 1 v)
+  (at level 20, t at level 50, format "l  ↦[ t ]  v") : bi_scope.
+
+Section liftable.
+
+  Context `{Σ : gFunctors}.
+  Context `{L : Type}.
+  Context `{V : Type}.
+  Context `{!EqDecision L}.
+  Context `{!Countable L}.
+
+  Definition heapT := @gen_heapG L V Σ _ _.
+
+  Lemma mapsto_disjoint h (a0 a1 : L) (v0 v1 : V) :
+    ( mapsto (Σ := Σ) (hG := h) a0 1 v0 -∗
+      mapsto (Σ := Σ) (hG := h) a1 1 v1 -∗
+      ⌜ a0 ≠ a1 ⌝ )%I.
+  Proof.
+    iIntros "Ha0 Ha1".
+    unfold mapsto.
+    rewrite seal_eq.
+    unfold mapsto_def.
+    iDestruct (own_valid_2 with "Ha0 Ha1") as "Ha".
+    generalize (@to_agree (leibnizO V) v0); intros.
+    generalize (@to_agree (leibnizO V) v1); intros.
+    iPure "Ha" as Ha.
+    iPureIntro.
+    destruct (decide (a0 = a1)); auto; subst.
+    exfalso.
+    (* ??? *)
+  Admitted.
+
+  Lemma big_sepM_disjoint h (m0 m1 : gmap L V) :
+    ( ( [∗ map] a↦v ∈ m0, mapsto (Σ := Σ) (hG := h) a 1 v ) -∗
+      ( [∗ map] a↦v ∈ m1, mapsto (Σ := Σ) (hG := h) a 1 v ) -∗
+      ⌜ m0 ##ₘ m1 ⌝ )%I.
+  Proof.
+    iIntros "H0 H1".
+    iIntros (i).
+    unfold option_relation.
+    destruct (m0 !! i) eqn:H0; destruct (m1 !! i) eqn:H1; try solve [ iPureIntro; auto ].
+    iDestruct (big_sepM_lookup with "H0") as "H0"; eauto.
+    iDestruct (big_sepM_lookup with "H1") as "H1"; eauto.
+    iDestruct (mapsto_disjoint with "H0 H1") as %Hc.
+    congruence.
+  Qed.
+
+  Class Liftable (P : heapT -> iProp Σ) := liftable :
+    ( ∀ h1, P h1 -∗
+      ∃ (m : gmap L V), ([∗ map] a ↦ v ∈ m, mapsto (Σ := Σ) (hG := h1) a 1 v) ∗
+           ∀ h2, ([∗ map] a ↦ v ∈ m, mapsto (Σ := Σ) (hG := h2) a 1 v) -∗ P h2
+    )%I.
+
+  Global Instance star_liftable `{Liftable P} `{Liftable Q} : Liftable (fun h => P h ∗ Q h)%I.
+  Proof.
+    unfold Liftable in *.
+    iIntros (?) "[Hp Hq]".
+    iDestruct (H with "Hp") as (mp) "[Hpm Hpi]".
+    iDestruct (H0 with "Hq") as (mq) "[Hqm Hqi]".
+    iExists (mp ∪ mq).
+    iDestruct (big_sepM_disjoint with "[$Hpm] [$Hqm]") as %?.
+    iDestruct (big_sepM_union with "[$Hpm $Hqm]") as "Hm"; eauto.
+    iFrame.
+    iIntros (h2) "Hm".
+    rewrite big_sepM_union; eauto.
+    iDestruct "Hm" as "[Hpm Hqm]".
+    iDestruct ("Hpi" with "Hpm") as "Hp".
+    iDestruct ("Hqi" with "Hqm") as "Hq".
+    iFrame.
+  Qed.
+
+  Global Instance pure_liftable P : Liftable (fun h => ⌜ P ⌝)%I.
+  Proof.
+    unfold Liftable in *.
+    iIntros (?) "%".
+    iExists ∅.
+    rewrite big_sepM_empty.
+    iSplit; try done.
+    iIntros (h2) "Hm".
+    iPureIntro. auto.
+  Qed.
+
+  Global Instance exists_liftable T P :
+    (forall x, Liftable (P x)) ->
+    Liftable (fun h => ∃ (x : T), P x h)%I.
+  Proof.
+    unfold Liftable in *.
+    iIntros (H h) "H".
+    iDestruct "H" as (x) "H".
+    iDestruct (H with "H") as (m) "(Hm & Hx)".
+    iExists _. iFrame.
+    iIntros (h2) "Hm".
+    iDestruct ("Hx" with "Hm") as "Hp".
+    iExists _. iFrame.
+  Qed.
+
+  Global Instance map_liftable `{EqDecision LM} `{Countable LM} `(m : gmap LM VM) P :
+    (forall a v, Liftable (P a v)) ->
+    Liftable (fun h => [∗ map] a ↦ v ∈ m, (P a v h))%I.
+  Proof.
+    intros.
+    unfold Liftable.
+    iIntros (?) "Hm".
+    iInduction m as [|i x m] "IH" using map_ind.
+    - iExists ∅.
+      repeat rewrite big_sepM_empty.
+      iFrame.
+      iIntros.
+      repeat rewrite big_sepM_empty.
+      done.
+    - iDestruct (big_sepM_insert with "Hm") as "[Hx Hm]"; auto.
+      iDestruct ("IH" with "Hm") as (m0) "[Hm0 Hr0]".
+      specialize (H0 i x).
+      unfold Liftable in H0.
+      iPoseProof H0 as "Hlift".
+      iDestruct ("Hlift" with "Hx") as (m1) "[Hm1 Hr1]".
+      iExists (m0 ∪ m1).
+      iDestruct (big_sepM_disjoint with "[$Hm0] [$Hm1]") as %?.
+      rewrite big_sepM_union; auto. iFrame.
+      iIntros (h2) "Hh2".
+      rewrite big_sepM_union; auto.
+      iDestruct ("Hh2") as "[Hm0 Hm1]".
+      iDestruct ("Hr0" with "Hm0") as "Hr0".
+      iDestruct ("Hr1" with "Hm1") as "Hr1".
+      rewrite big_sepM_insert; auto.
+      iFrame.
+  Qed.
+
+  Global Instance mapsto_liftable :
+    Liftable (fun h => a ↦[h] v)%I.
+  Proof.
+    intros; unfold Liftable.
+    iIntros (h1) "Ha".
+    iExists (<[a:=v]> ∅).
+    rewrite big_sepM_insert.
+    iFrame.
+    rewrite big_sepM_empty.
+    iSplitL. done.
+    iIntros (h2) "Hh2".
+    rewrite big_sepM_insert.
+    iDestruct "Hh2" as "[Ha Hemp]".
+    rewrite big_sepM_empty.
+    iFrame.
+    apply lookup_empty.
+    apply lookup_empty.
+  Qed.
+
+  Global Instance emp_liftable : Liftable (fun h => emp)%I.
+  Proof.
+    intros; unfold Liftable.
+    iIntros (h1) "H".
+    iExists ∅.
+    rewrite big_sepM_empty; iFrame.
+    iIntros (h2) "Hm".
+    rewrite big_sepM_empty; iFrame.
+  Qed.
+
+  Lemma list_liftable' `(l : list V) off P :
+    (forall a v, Liftable (P a v)) ->
+    Liftable (fun h => [∗ list] a ↦ v ∈ l, (P (off + a) v h))%I.
+  Proof.
+    intros.
+    generalize dependent off.
+    induction l; intros.
+    - apply emp_liftable.
+    - unfold Liftable in *.
+      iIntros (h1) "[Ha Hl]".
+      iDestruct (H with "Ha") as (ma0) "[Ha Hm0]".
+      setoid_rewrite <- plus_n_Sm.
+      setoid_rewrite <- plus_Sn_m.
+      iDestruct (IHl with "Hl") as (ml) "[Hl Hml]".
+      iExists (ma0 ∪ ml).
+      iDestruct (big_sepM_disjoint with "[$Ha] [$Hl]") as %?.
+      rewrite big_sepM_union; auto; iFrame.
+      iIntros (h2) "Hh2".
+      rewrite big_sepM_union; auto.
+      iDestruct "Hh2" as "[Ha Hl]".
+      iDestruct ("Hm0" with "Ha") as "Ha".
+      iDestruct ("Hml" with "Hl") as "Hl".
+      simpl.
+      setoid_rewrite <- plus_n_Sm.
+      setoid_rewrite <- plus_Sn_m.
+      iFrame.
+  Qed.
+
+  Global Instance list_liftable `(l : list V) P :
+    (forall a v, Liftable (P a v)) ->
+    Liftable (fun h => [∗ list] a ↦ v ∈ l, (P a v h))%I.
+  Proof.
+    intros.
+    apply (list_liftable' l 0 P) in H.
+    simpl in H.
+    auto.
+  Qed.
+
+End liftable.
